fixes to make the proof succeed

proof/memory_map.bpl
@@ -36,15 +36,17 @@ const sir_channel_context_ptr_high : uint8_ptr_t; axiom sir_channel_context_ptr_
 
 /*************** lot of empty space ****************/
 var heap_base: mem_t;
-const heap_base_ptr_low: uint8_ptr_t;        axiom heap_ptr_low == 16384bv64;
-const heap_base_ptr_high: uint8_ptr_t;       axiom heap_ptr_high == 16400bv64;
+const heap_base_ptr_low: uint8_ptr_t;        axiom heap_base_ptr_low == 16384bv64;
+const heap_base_ptr_high: uint8_ptr_t;       axiom heap_base_ptr_high == 16400bv64;
 
 var freep: header_ptr_t; //TODO: put this in memory
 
 var heap: mem_t; //from 12288bv64 to 16384bv64
 const heap_ptr_low: uint8_ptr_t;        axiom heap_ptr_low == 12288bv64;
 const heap_ptr_high: uint8_ptr_t;       axiom heap_ptr_high == 16384bv64;
+const heap_size: uint8_ptr_t;           axiom heap_size == 4096bv64;
 function {:inline} AddrInHeap(x: bv64): bool { GE_64(x, heap_ptr_low) && LT_64(x, heap_ptr_high) }
+function {:inline} AddrInHeapInclusive(x: bv64): bool { GE_64(x, heap_ptr_low) && LE_64(x, heap_ptr_high) }
 
 var stack: mem_t; //from 8192bv64 to 12288bv64
 const stack_ptr_low: uint8_ptr_t;        axiom stack_ptr_low == 8192bv64;
