proof/U.bpl
@@ -1,5 +1,5 @@
 procedure U( )
-//modifies mem;
+modifies U;
 {
-
+  havoc U;
 }
