proof/verified_L.bpl
@@ -11,6 +11,7 @@ modifies send_buf, recv_buf, stack, stack_guard, freep, sir_heap_context,
   call init_channel(send_buf_ptr_low, send_buf_size,
                     recv_buf_ptr_low, recv_buf_size,
                     symmetric_key_ptr_low);
+  call init_heap(heap_ptr_low, heap_size);
 
   while(*)
   invariant AddrInSendBuf(LOAD_LE_64(sir_channel_context, PLUS_64(sir_channel_context_ptr_low, 16bv64)));
@@ -18,14 +19,19 @@ modifies send_buf, recv_buf, stack, stack_guard, freep, sir_heap_context,
                        PLUS_64(sir_channel_context_ptr_low, 8bv64)) == send_buf_size;
   invariant LOAD_LE_64(sir_channel_context,
                        PLUS_64(sir_channel_context_ptr_low, 0bv64)) == send_buf_ptr_low;
+  invariant AddrInHeapInclusive(LOAD_LE_64(sir_heap_context, PLUS_64(sir_heap_context_ptr_low, 16bv64)));
+  invariant LOAD_LE_64(sir_heap_context,
+                      PLUS_64(sir_heap_context_ptr_low, 8bv64)) == heap_size;
+  invariant LOAD_LE_64(sir_heap_context,
+                      PLUS_64(sir_heap_context_ptr_low, 0bv64)) == heap_ptr_low;
   {
     havoc buf;
     havoc size;
 
     if (*) { call U(); }
     else if (*) { call heap_result, malloc_region := L_malloc(size); }
-    else if (*) { call heap_result := L_free(buf); }
+    //else if (*) { call heap_result := L_free(buf); }
     else if (*) { call channel_result := L_send(buf,size); }
-    else if (*) { call channel_result := L_recv(buf,size); }
+    //else if (*) { call channel_result := L_recv(buf,size); }
   }
 }
